src/Cvm_Impl.v
@@ -11,37 +11,43 @@ Import ListNotations.
 
 (** Monadic VM implementation *)
 
-Fixpoint copland_compile (t:AnnoTermPar): CVM unit :=
+Fixpoint copland_compile (t:Core_Term): CVM unit :=
   match t with
-  | aasp_par a =>
+  | aspc a =>
       e <- do_prim a ;;
       put_ev e
-  | aatt_par q t' =>
+  | attc q t' =>
     e <- get_ev ;;
     e' <- doRemote t' q e ;;
     put_ev e'
-  | alseq_par t1 t2 =>
+  | lseqc t1 t2 =>
       copland_compile t1 ;;
       copland_compile t2
-  | abseq_par sp t1 t2 =>
+  | bseqc t1 t2 =>
+    (*
     pr <- split_ev sp ;;
     let '(e1,e2) := pr in
-    put_ev e1 ;;
+    put_ev e1 ;; *)
+    split_ev ;;
+    e <- get_ev ;;
     copland_compile t1 ;;
     e1r <- get_ev ;;
-    put_ev e2 ;;
+    put_ev e ;;
     copland_compile t2 ;;
     e2r <- get_ev ;;
     join_seq e1r e2r
-  | abpar_par loc sp t1 t2 =>
+  | bparc loc t1 t2 =>
+    split_ev ;;
+    e <- get_ev ;;
+    (*
     pr <- split_ev sp ;;
-    let '(e1,e2) := pr in
-    start_par_thread loc t2 e2 ;;
-    put_ev e1 ;;
+    let '(e1,e2) := pr in *)
+    start_par_thread loc t2 e ;;
+    (* put_ev e1 ;; *)
     copland_compile t1 ;;
     e1r <- get_ev ;;
-    e2r <- wait_par_thread loc t2 e2 ;;
-    join_par e1r e2r
+    e2r <- wait_par_thread loc t2 e ;;
+    join_seq e1r e2r
   end.
 
 (*
