src/Evidence_Bundlers.v
@@ -5,19 +5,22 @@ Import ListNotations.
 
 (* Matches on evidence type param only for verification.  
    Will extract to the cons function over the first two params (new measurement bits + existing evidence) *)
+
+(*
 Definition cons_uu (x:BS) (e:EvC) (*(i:ASP_ID) (args:list Arg) (tpl:Plc) (tid:TARG_ID) (tet:Evidence)*)(params:ASP_PARAMS) (mpl:Plc) : EvC :=
   match e with
   | evc bits et => evc (x :: bits) (uu params(*i args tpl tid tet*) mpl et)
   end.
+*)
 
-Definition cons_sig (sig:BS) (e:EvC) (p:Plc): EvC :=
+Definition cons_gg (sig:BS) (e:EvC) (p:Plc) (ps:ASP_PARAMS): EvC :=
   match e with
-  | evc bits et => evc (sig :: bits) (gg p et)
+  | evc bits et => evc (sig :: bits) (gg p ps et)
   end.
 
-Definition cons_hh (hsh:BS) (e:EvC) (p:Plc): EvC :=
+Definition cons_hh (hsh:BS) (e:EvC) (p:Plc) (ps:ASP_PARAMS): EvC :=
   match e with
-  | evc _ et => evc [hsh] (hh p et)
+  | evc _ et => evc [hsh] (hh p ps et)
   end.
 
 Definition ss_cons (e1:EvC) (e2:EvC): EvC :=
@@ -25,10 +28,13 @@ Definition ss_cons (e1:EvC) (e2:EvC): EvC :=
   | (evc bits1 et1, evc bits2 et2) => evc (bits1 ++ bits2) (ss et1 et2)
   end.
 
+(*
+
 Definition pp_cons (e1:EvC) (e2:EvC): EvC :=
   match (e1, e2) with
   | (evc bits1 et1, evc bits2 et2) => evc (bits1 ++ bits2) (pp et1 et2)
   end.
+*)
 
 Definition encodeEvBits (e:EvC): BS :=
   match e with
